Test/VProg.v
@@ -9,10 +9,10 @@ Section Program.
   Variable (CT : CP.context).
 
 
-Definition spec_0 : FDecl (ptr * ptr) _ unit _
-  SPEC (p0, p1)
+Definition spec_0 : FDecl SPEC
+  ((p0, p1) : ptr * ptr)
   '(n0, n1) [] [vptr p0 ~> n0; vptr p1 ~> n1] True
-  '_ tt [vptr p0 ~> n1; vptr p1 ~> n0] True.
+  '(_ : unit) tt [vptr p0 ~> n1; vptr p1 ~> n0] True.
 Proof. Derived. Defined.
 Variable f_0 : spec_0 CT.
 
@@ -25,10 +25,10 @@ Lemma correct_0 : FCorrect vprog_0.
 Proof. solve_by_wlp. Qed.
 
 
-Definition spec_1 : FDecl (ptr * ptr * ptr) _ unit _
-  SPEC (p0, p1, p2)
+Definition spec_1 : FDecl SPEC
+  ((p0, p1, p2) : ptr * ptr * ptr)
   '(n0, n1, n2) [vptr p2 ~> n2] [vptr p0 ~> n0; vptr p1 ~> n1] True
-  '_ tt [vptr p0 ~> n1; vptr p1 ~> n0] True.
+  '(_ : unit) tt [vptr p0 ~> n1; vptr p1 ~> n0] True.
 Proof. Derived. Defined.
 Variable f_1 : spec_1 CT.
 
@@ -40,10 +40,10 @@ Proof. solve_by_wlp. Qed.
 
 Definition data42 : nat := 42.
 
-Definition spec_2 : FDecl (ptr * ptr * ptr) _ ptr _
-  SPEC (p0, p1, p2)
+Definition spec_2 : FDecl SPEC
+  ((p0, p1, p2) : ptr * ptr * ptr)
   '(n0, n1, n2) [vptr p2 ~> n2] [vptr p0 ~> n0; vptr p1 ~> n1] True
-  'p (n, n1') [vptr p ~> n; vptr p1 ~> n1'] (n1' > 0).
+  '(p : ptr) (n, n1') [vptr p ~> n; vptr p1 ~> n1'] (n1' > 0).
 Proof. Derived. Defined.
 Variable f_2 : spec_2 CT.
 
@@ -60,10 +60,10 @@ Proof.
 Qed.
 
 
-Definition spec_3 : FDecl ptr (Some (fun _ => ptr)) ptr (Some (fun _ => ptr))
-  SPEC p0 & p1
+Definition spec_3 : FDecl SPEC
+  (p0 : ptr) & (p1 : ptr)
   '(n0, n1) [] [vptr p0 ~> n0; vptr p1 ~> n1] True
-  'p0' & p1' (n0', n1') [vptr p0' ~> n0'; vptr p1' ~> n1'] True.
+  '(p0' : ptr) & (p1' : ptr) (n0', n1') [vptr p0' ~> n0'; vptr p1' ~> n1'] True.
 Proof. Derived. Defined.
 Variable f_3 : spec_3 CT.
 
@@ -73,10 +73,10 @@ Lemma correct_3: FCorrect vprog_3.
 Proof. solve_by_wlp. Qed.
 
 
-Definition spec_4 : FDecl (ptr * ptr) _ ptr (Some (fun _ => ptr))
-  SPEC (p0, p1)
+Definition spec_4 : FDecl SPEC
+  ((p0, p1) : ptr * ptr)
   '(n0, n1) [] [vptr p0 ~> n0; vptr p1 ~> n1] True
-  'p0' & p1' (n0', n1') [vptr p0' ~> n0'; vptr p1' ~> n1'] True.
+  '(p0' : ptr) & (p1' : ptr) (n0', n1') [vptr p0' ~> n0'; vptr p1' ~> n1'] True.
 Proof. Derived. Defined.
 Variable f_4 : spec_4 CT.
 
@@ -90,9 +90,9 @@ Proof. solve_by_wlp. Qed.
 Definition cell2 (p : ptr) '(v0, v1) : SLprop.t :=
   (SLprop.cell p v0 ** SLprop.cell (S p) v1)%slprop.
 
-Definition elim_cell2_spec : LDecl ptr unit
-  SPEC p 'n01 [] [cell2 p ~> n01] True
-  '_ tt [vptr p ~> (fst n01); vptr (S p) ~> (snd n01)] True.
+Definition elim_cell2_spec : LDecl SPEC
+  (p : ptr) 'n01 [] [cell2 p ~> n01] True
+  '(_ : unit) tt [vptr p ~> (fst n01); vptr (S p) ~> (snd n01)] True.
 Proof. Derived. Defined.
 Lemma elim_cell2 : elim_cell2_spec.
 Proof.
@@ -100,9 +100,9 @@ Proof.
   reflexivity.
 Qed.
 
-Definition intro_cell2_spec : LDecl ptr unit
-  SPEC p '(n0, n1) [] [vptr p ~> n0; vptr (S p) ~> n1] True
-  '_ tt [cell2 p ~> (n0, n1)] True.
+Definition intro_cell2_spec : LDecl SPEC
+  (p : ptr) '(n0, n1) [] [vptr p ~> n0; vptr (S p) ~> n1] True
+  '(_ : unit) tt [cell2 p ~> (n0, n1)] True.
 Proof. Derived. Defined.
 Lemma intro_cell2 : intro_cell2_spec.
 Proof.
@@ -110,9 +110,9 @@ Proof.
   reflexivity.
 Qed.
 
-Definition spec_5 : FDecl ptr _ unit _
-  SPEC p 'v [] [cell2 p ~> v] True
-  '_ v' [cell2 p ~> v'] (v' = let (n0, n1) := v in (S n0, n1)).
+Definition spec_5 : FDecl SPEC
+  (p : ptr) 'v [] [cell2 p ~> v] True
+  '(_ : unit) v' [cell2 p ~> v'] (v' = let (n0, n1) := v in (S n0, n1)).
 Proof. Derived. Defined.
 Variable f_5 : spec_5 CT.
 
@@ -125,9 +125,9 @@ Lemma correct_5: FCorrect vprog_5.
 Proof. solve_by_wlp. Qed.
 
 
-Definition spec_f0 : FDecl ptr _ (nat * nat) _
-  SPEC p 'v [cell2 p ~> v] [] True
-  'r tt [] (@eq (nat*nat) r v).
+Definition spec_f0 : FDecl SPEC
+  (p : ptr) 'v [cell2 p ~> v] [] True
+  '(r : nat * nat) tt [] (r = v).
 Proof. Derived. Defined.
 
 Definition vfrag_0_impl : FragImpl spec_f0 CT :=
@@ -143,9 +143,9 @@ Proof.
   case sel0; reflexivity.
 Qed.
 
-Definition spec_6 : FDecl ptr _ nat _
-  SPEC p 'v [cell2 p ~> v] [] True
-  'n tt [] (n = fst v).
+Definition spec_6 : FDecl SPEC
+  (p : ptr) 'v [cell2 p ~> v] [] True
+  '(n : nat) tt [] (n = fst v).
 Proof. Derived. Defined.
 Variable f_6 : spec_6 CT.
 
@@ -173,8 +173,8 @@ Section Other.
 
 Definition sigh_a0 := mk_f_sig1 (ptr * ptr) None unit None.
 Definition spec_a0 : FSpec sigh_a0
-  SPEC ps 'n [vptr (fst ps) ~> n] [] True
-  '_ tt [] True.
+  SPEC (ps : _) 'n [vptr (fst ps) ~> n] [] True
+  '(_ : _) tt [] True.
 Proof. Tac.build_FSpec. Defined.
 
 Definition vprog_a0 : f_body CT sigh_a0 := fun ps =>
@@ -190,9 +190,9 @@ Proof. Tac.extract_impl. Defined.
 
 Definition sigh_a1a := mk_f_sig1 (bool * ptr * ptr * ptr) None unit None.
 Definition spec_a1a : FSpec sigh_a1a
-  SPEC (b, p0, p1, p2)
+  SPEC ((b, p0, p1, p2) : _)
   '(n0, n1, n2) [vptr p0 ~> n0] [vptr p1 ~> n1; vptr p2 ~> n2] True
-  '_ (n1', n2') [vptr p1 ~> n1'; vptr p2 ~> n2'] (b = true -> n1' = 0).
+  '(_ : _) (n1', n2') [vptr p1 ~> n1'; vptr p2 ~> n2'] (b = true -> n1' = 0).
 Proof. Tac.build_FSpec. Defined.
 
 Definition vprog_a1a : f_body CT sigh_a1a := fun '(b, p0, p1, p2) =>
@@ -211,9 +211,9 @@ Inductive bool3 : Set := B0 | B1 | B2.
 
 Definition sigh_a1b := mk_f_sig1 (bool3 * ptr) None unit None.
 Definition spec_a1b : FSpec sigh_a1b
-  SPEC (b, p)
+  SPEC ((b, p) : _)
   'n [] [vptr p ~> n] (b <> B2)
-  '_ n' [vptr p ~> n'] (b <> B1 -> n' = 0).
+  '(_ : _) n' [vptr p ~> n'] (b <> B1 -> n' = 0).
 Proof. Tac.build_FSpec. Defined.
 
 Definition vprog_a1b : f_body CT sigh_a1b := fun '(b, p) =>
@@ -228,9 +228,9 @@ Proof. solve_by_wlp; congruence. Qed.
 
 Definition sigh_a1c := mk_f_sig1 (option nat * ptr) None unit None.
 Definition spec_a1c : FSpec sigh_a1c
-  SPEC (o, p)
+  SPEC ((o, p) : _)
   'n [] [vptr p ~> n] (n > 0 /\ match o with Some n' => n' > 0 | None => True end)
-  '_ n' [vptr p ~> n'] (n' > 0).
+  '(_ : _) n' [vptr p ~> n'] (n' > 0).
 Proof. Tac.build_FSpec. Defined.
 
 Definition vprog_a1c : f_body CT sigh_a1c := fun '(o, p) =>
@@ -245,9 +245,9 @@ Proof. solve_by_wlp. Qed.
 
 Definition sigh_a2a := mk_f_sig1 (ptr * ptr) None unit None.
 Definition spec_a2a : FSpec sigh_a2a
-  SPEC (p0, p1)
+  SPEC ((p0, p1) : _)
   '(n0, n1) [vptr p0 ~> n0] [vptr p1 ~> n1] (n0 <= n1)
-  '_ n1' [vptr p1 ~> n1'] (n0 <= n1').
+  '(_ : _) n1' [vptr p1 ~> n1'] (n0 <= n1').
 Proof. Tac.build_FSpec. Defined.
 
 Definition vprog_a2a : f_body CT sigh_a2a := fun '(p0, p1) =>
@@ -277,9 +277,9 @@ Proof. Tac.extract_impl. Defined.
 
 Definition sigh_a3 := mk_f_sig1 unit (Some (fun _ => (nat * nat)%type <: Type)) unit (Some (fun _ => nat <: Type)).
 Definition spec_a3 : FSpec sigh_a3
-  SPEC _ & (n0, n1)
+  SPEC (_ : _) & ((n0, n1) : _)
   'tt [] [] True
-  '_ & r tt [] (r = n0 + n1).
+  '(_ : _) & (r : _) tt [] (r = n0 + n1).
 Proof. Tac.build_FSpec. Defined.
 
 Definition vprog_a3 : f_body CT sigh_a3 := fun _ '(n0, n1) =>
